
# 10.5      Extension Fields 

![[DMath-e-u10.pdf#page=1&rect=78,193,522,212|DMath-e-u10, p.1]]

## a) ![[DMath-e-u10.pdf#page=1&rect=105,178,522,193|DMath-e-u10, p.1]]

The algebra $\mathbb{Z}_{3}$ is a commutative ring, by example 5.34. Then, by theorem 5.21, if $R$ is a commutative ring, the extension $R[x]$ is also a commutative ring. Thus the structure $\mathbb{Z}_{3}[x]$ is a non-trivial commutative ring, since the additive and multiplicative identity are distinct, $\mathbf{0}\neq \mathbf{1}$. Per lemma 5.35, $F[x]_{m(x)}$ is a ring with respect to addition and multiplication. Thus the algebra $\mathbb{Z}_{3}[x]_{x^{3}+2x^{2}+1}$ is a ring.

Finally, for a ring $F$ its extension field $F[x]_{m(x)}$ is a field if and only if $m(x)$ is irreducible, by theorem 5.37. Thus all that remains to show is that $m(x) = x^{3}+2x^{2}+1$ is irreducible in $\mathbb{Z}_{3}[x]$.

To do this, it follows from definition 5.28 and the fact that degrees of polynomials are added under multiplication. Since the degree of the modulus polynomial is three $\deg(m(x))=3$, it suffices to prove that it has no monic polynomial divisors. This can be expressed as $(x-\alpha) \not\equiv_{m(x)} 0$ for all $\alpha \in \mathbb{Z}_{3}$. Computations yield the following.
$$
\begin{align}
R_{x+0}(x^{3}+2x^{2}+1) &= 1 \\
R_{x+1}(x^{3}+2x^{2}+1) &= 2 \\
R_{x+2}(x^{3}+2x^{2}+1) &= 1
\end{align}
$$

Thus, $m(x) = x^{3}+2x^{2}+1$ is an irreducible polynomial in $\mathbb{Z}_{3}[x]$ and hence $F = \mathbb{Z}_{3}[x]_{x^{3}+2x^{2}+1}$ is a field.
$\square$

<div class="page-break" style="page-break-before: always;"></div>

## b) ![[DMath-e-u10.pdf#page=1&rect=106,159,522,174|DMath-e-u10, p.1]]

Recall that $F^{*}$ is the (cyclic) group of units in the finite field $F$. Its order is given by the following.
$$
\begin{align}
|F^{*}| &= |F - \{ 0 \}| &\text{(D. 5.26.)} \\
&= |F| -1 &\text{(L. 5.34.)} \\
&= |\mathbb{Z}_{3}|^{\deg(m(x))} - 1 \\
&=3^{3}-1  \\
&= 26
\end{align}
$$

The elements of $F^{*}$ are polynomials of the form $a(x) = \alpha_{2}x^{2} + \alpha_{1}x + \alpha_{0}$, where $\alpha_{i} \in \mathbb{Z}_{3}$, not all equal zero. Since all constant polynomials only generate constant polynomials, let's consider the simplest monic polynomial with an indeterminate, $g(x) = x \in F^{*}$. The computations of the powers of $g(x)$ are given below.
$$
\begin{align}
g(x)^{0} = x^{0} &\equiv_{m(x)} 1 \\
g(x)^{1} = x^{1} &\equiv_{m(x)} x \\
g(x)^{2} = x^{2} &\equiv_{m(x)} x^{2} \\
g(x)^{3} = x^{3} &\equiv_{m(x)} x^{2} - 1 \\
g(x)^{4} = x^{4} &\equiv_{m(x)} x^{2} - x - 1 \\
g(x)^{5} = x^{5} &\equiv_{m(x)} -x - 1 \\
g(x)^{6} = x^{6} &\equiv_{m(x)} -x^{2} - x \\
g(x)^{7} = x^{7} &\equiv_{m(x)} x^{2} + 1 \\
g(x)^{8} = x^{8} &\equiv_{m(x)} x^{2} + x - 1 \\
g(x)^{9} = x^{9} &\equiv_{m(x)} -x^{2} - x - 1 \\
g(x)^{10} = x^{10} &\equiv_{m(x)} x^{2} - x + 1 \\
g(x)^{11} = x^{11} &\equiv_{m(x)} x - 1 \\
g(x)^{12} = x^{12} &\equiv_{m(x)} x^{2} - x &= - g(x)^{-1} \\
g(x)^{13} = x^{13} &\equiv_{m(x)} - 1 &= -g(x)^{0} \ \ \\
g(x)^{14} = x^{14} &\equiv_{m(x)} - x &= - g(x)^{1} \ \ \\
g(x)^{15} = x^{15} &\equiv_{m(x)} -x^{2} &=-g(x)^{2} \ \ \\
& \phantom{x} \vdots & \vdots \qquad\qquad \\
g(x)^{25} = x^{25} &\equiv_{m(x)} -x^{2} + x &= g(x)^{-1} \ \ \ \\
g(x)^{26} = x^{26} &\equiv_{m(x)} 1
\end{align}
$$

It can be observed, that after the first thirteen iterations, continued exponentiation repeats the additive inverses of the previous expressions. Thus, since it holds that $\langle x \rangle = F^{*}$, the polynomial $g(x) = x$ is a generator of$F^{*}$.

An alternative approach is given as follows. By lagrange's theorem (T. 5.8.), for a finite group $G$ and subgroup $H$ it holds that  the order of $H$ divides the order of $G$.

Let $H = \langle x \rangle \subseteq F^{*}$ be the subgroup generated by the postulated generator $x$. Thus it must be true that $|H| \in \{ 1, 2, 13, 26 \}$, since those are the possible orders that divide the order of $|F^{*}|=26$. Then per corollary 5.10, we know that $x^{|H|} = 1$, since trivially $x \in H$. Then, for $n \in \{ 1, 2, 13 \}$ we have $x^{n} \neq 1$ as shown below.
$$
\begin{align}
x^{1} &\equiv_{m(x)} x \\
x^{2} &\equiv_{m(x)} x^{2} \\
x^{13} &\equiv_{m(x)} 2
\end{align}
$$

However, we have $x^{26} \equiv_{m(x)} 1$. Thus, since the order of the subgroup generated by $x$ is equal to that of the multiplicative group of the underlying field, $|H| = 26 = |F^{*}|$ and the subgroup is a subset of the multiplicative group of units $H \subseteq F^{*}$, it must be that $H = F^{*}$. Hence $x$ is a generator of $F^{*}$.
$\square$

<div class="page-break" style="page-break-before: always;"></div>

# c) ![[DMath-e-u10.pdf#page=1&rect=106,140,522,156|DMath-e-u10, p.1]]

Recall that $F$ is the field of polynomials in $x$ with coefficients in $\mathbb{Z}_{3}$ and degree less than three. Then $F[y]$ is the ring of polynomials in $y$ with coefficients in $F$. 

Per theorem 5.31, since $F$ is a field, the non-zero polynomial $a(y) \in F[y]$ of degree $d=2$ has at most two roots, i.e. an element $\alpha \in F$ such that $a(\alpha) = 0$. This implies that $a(\alpha) \equiv_{m(x)} m(x)$. Then we can rewrite $a(y)$ as given below.
$$
\begin{align}
a(y) = y^{2} + 2y(x^{2} + x) + (x^{2} + 2) &\equiv_{m(x)} x^{3} - x^{2} + 1 &\text{(associativity)} \\
y^{2} - yx^{2} - yx + x^{2} + 2 &\equiv_{m(x)} x^{3} - x^{2} + 1 &  (- x^{2} - 2) \\
y^{2} - yx^{2} - yx &\equiv_{m(x)} x^{3} + x^{2} - 1 &(x^{2} -1 \equiv_{m(x)} x^{3}) \\
 &\equiv_{m(x)} -x^{3} \\
\end{align}
$$
First, let's consider the element $\alpha_{1} = x \in F$. Evaluation confirms that this is a root, since it holds that $a(\alpha_{1}) = \cancel{ x^{2} - x^{2} } -x^{3}$, through commutativity and definition of the additive inverse.

Second, observe $\alpha_{2} = x^{2} \in F$. Computation of the polynomial yields $a(\alpha_{2}) = \cancel{ x^{4} - x^{4} } -x^{3}$. As above, it holds that the polynomial at $\alpha_{2}$ is congruent to zero modulo $m(x)$.



%%
Since $F$ is a field, and by theorem 5.24, every field is an integral domain, $F[y]$ is an integral domain by lemma 5.22. Its elements are the polynomials in $y$ with coefficients in $F = \mathbb{Z}_{3}[x]_{m(x)}$. This can alternatively be understood as the polynomials in two indeterminates i.e. $a(x,y) \in \mathbb{Z}_{3}[x, y]_{m(x)}$, as in example 5.43. Then, per definition 5.33 for a polynomial $a(x,y) \in \mathbb{Z}_{3}[x,y]_{m(x)}$ an element $(\alpha, \beta) \in \mathbb{Z}_{3} \times \mathbb{Z}_{3}$ is a root exactly when $a(\alpha, \beta) = 0$. The following table presents the evaluation of $a(x,y)$ for all $(\alpha, \beta) \in \mathbb{Z}_{3} \times \mathbb{Z}_{3}$. The roots are marked.
$$
\begin{array}{c | c | c  | c}
a(x, y) & \beta=0 & \beta=1 & \beta=2 \\
\hline
\alpha=0 & 2 & \boxed{0} & \boxed{0} \\
\hline
\alpha=1 & \boxed{0} & 1 & \boxed{0} \\
\hline
\alpha=2 & \boxed{0} & 1 & 1
\end{array}
$$
$\square$
%%




