---
"course:": "[[DMath]]"
"exercises:": "[[DMath_U2_e.pdf]]"
"hand-in:": "[[DMath_U2_bf.pdf]]"
"solutions:": "[[DMath_U2_s.pdf]]"
---
Two ways to understand
$F=\forall A(x=0 \vee \exists y (x\cdot y = 1))$

- w/o interpretation (universe, predicates, what is equal?):
	$F \equiv \forall x (\lnot\lnot (x=0) \vee \exists y (x\cdot y = 1))$
	$F \equiv \forall x (\lnot (x=0) \rightarrow \exists y (x\cdot y = 1))$

-with interpretation:
	every number that is not zero has a multiplicative inverse
	valid (Q, R)
	invalid (N, Z)


>$\exists x (P(x) \wedge Q(x))$
>$\exists x P(x) \wedge \exists x Q(x)$
>
>$\exists x (P(x) \wedge Q(x)) \models \exists x P(x) \wedge \exists x Q(x)$
>$\exists x P(x) \wedge \exists x Q(x) \nVdash \exists x (P(x) \wedge Q(x))$


>[!example] Definitions:
>"$\models$": F is true if P($\alpha$) and Q($\alpha$) for some (same) $\alpha \exists \mathbb{U}$
>Then there's an x($\alpha$) so that P(x) true
>**and** an x($\alpha$) so that Q(x) true
>
>"$\nVdash$": Let U=$\mathbb{N}$, P(x) $\overset{def.}{\Leftrightarrow}$ even(x), Q(x)$\overset{def.}{\Leftrightarrow}$ odd(x)
>Then G is true but F isn't.


- $\exists x (F \wedge G) \equiv \exists x F \vee \exists x G$
- $\forall (F \wedge G) \equiv \forall x F \wedge \forall x G$
- $\forall x /F \vee G) \nVdash \forall x F \vee \forall x G$
- $\lnot \forall x F \equiv \exists x \lnot F, \lnot \exists x F \equiv \forall x \lnot F$
- $\exists x \exists y F \equiv \exists y \exists x F$
- $\forall x \forall y F \equiv \forall y \forall x F$

- $\exists y \forall x F \models \forall x \exists y F$
- $\forall x \exists y F \nvDash \exists y \forall x F$


- F tautology  

- $F := \forall x P(x) \rightarrow \exists P(x)$
- $\quad\equiv \lnot \forall x P(x) \vee \exists x P(x)$ \[Def. $\rightarrow$]
- $\quad\equiv \exists x \lnot P(x) \vee \exists x P(x)$ \[2.4.8]
- $\quad\equiv\exists x (\lnot P(x) \vee P(x))$ \[Ch. 6]
- $\quad\equiv \exists x \top$
- $\quad\equiv\top$

>[!example] Just a formula, **not** a statement:
>$\exists x \forall y \, x \leq y, \, for \, U=\mathbb{N}, \leq on\, \mathbb{N}$ (true) statement
>(**false** statement) for $U=\mathbb{Z}$

>[!example] Composition of $\implies$
>If $S\implies T$ and $T\implies U$ are true, we condclude $S\implies U$ true as well.
>Proof: $(A\rightarrow B) \wedge (B\rightarrow C) \models A \rightarrow C$
>
>Variants: 




