
### Differentiation Rules
$$
\begin{aligned}
&\text{(Constant Rule)} & \frac{d}{dx} c &= 0 \\
&\text{(Power Rule)} & \frac{d}{dx} x^n &= nx^{n-1} \\
&\text{(Constant Multiple Rule)} & \frac{d}{dx} [c \cdot f(x)] &= c \cdot f'(x) \\
&\text{(Sum Rule)} & \frac{d}{dx} [f(x) + g(x)] &= f'(x) + g'(x) \\
&\text{(Difference Rule)} & \frac{d}{dx} [f(x) - g(x)] &= f'(x) - g'(x) \\
&\text{(Product Rule)} & \frac{d}{dx} [f(x) \cdot g(x)] &= f'(x) g(x) + f(x) g'(x) \\
&\text{(Quotient Rule)} & \frac{d}{dx} \left[\frac{f(x)}{g(x)}\right] &= \frac{f'(x) g(x) - f(x) g'(x)}{[g(x)]^2} \\
&\text{(Chain Rule)} & \frac{d}{dx} f(g(x)) &= f'(g(x)) \cdot g'(x) \\
&\text{(Exponential Rule)} & \frac{d}{dx} e^x &= e^x \\
&\text{(Logarithm Rule)} & \frac{d}{dx} \ln(x) &= \frac{1}{x} \\
&\text{(General Exponential Rule)} & \frac{d}{dx} a^x &= a^x \ln(a) \\
&\text{(General Logarithm Rule)} & \frac{d}{dx} \log_a(x) &= \frac{1}{x \ln(a)} \\
&\text{(Trigonometric Functions)} & \frac{d}{dx} \sin(x) &= \cos(x) \\
& & \frac{d}{dx} \cos(x) &= -\sin(x) \\
& & \frac{d}{dx} \tan(x) &= \sec^2(x) \\
& & \frac{d}{dx} \cot(x) &= -\csc^2(x) \\
& & \frac{d}{dx} \sec(x) &= \sec(x) \tan(x) \\
& & \frac{d}{dx} \csc(x) &= -\csc(x) \cot(x) \\
&\text{(Inverse Trigonometric Functions)} & \frac{d}{dx} \sin^{-1}(x) &= \frac{1}{\sqrt{1-x^2}} \\
& & \frac{d}{dx} \cos^{-1}(x) &= -\frac{1}{\sqrt{1-x^2}} \\
& & \frac{d}{dx} \tan^{-1}(x) &= \frac{1}{1+x^2} \\
& & \frac{d}{dx} \cot^{-1}(x) &= -\frac{1}{1+x^2} \\
& & \frac{d}{dx} \sec^{-1}(x) &= \frac{1}{|x| \sqrt{x^2-1}} \\
& & \frac{d}{dx} \csc^{-1}(x) &= -\frac{1}{|x| \sqrt{x^2-1}}
\end{aligned}
$$

### Integration Rules
$$
\begin{aligned}
&\text{(Constant Rule)} & \int c \, dx &= cx + C \\
&\text{(Power Rule)} & \int x^n \, dx &= \frac{x^{n+1}}{n+1} + C \quad (n \neq -1) \\
&\text{(Constant Multiple Rule)} & \int c \cdot f(x) \, dx &= c \int f(x) \, dx \\
&\text{(Sum Rule)} & \int [f(x) + g(x)] \, dx &= \int f(x) \, dx + \int g(x) \, dx \\
&\text{(Difference Rule)} & \int [f(x) - g(x)] \, dx &= \int f(x) \, dx - \int g(x) \, dx \\
&\text{(Integration by Parts)} & \int u \, dv &= uv - \int v \, du \\
&\text{(Substitution Rule)} & \int f(g(x)) g'(x) \, dx &= \int f(u) \, du \quad (u = g(x)) \\
&\text{(Exponential Rule)} & \int e^x \, dx &= e^x + C \\
&\text{(General Exponential Rule)} & \int a^x \, dx &= \frac{a^x}{\ln(a)} + C \\
&\text{(Logarithm Rule)} & \int \ln(x) \, dx &= x \ln(x) - x + C \\
&\text{(Trigonometric Functions)} & \int \sin(x) \, dx &= -\cos(x) + C \\
& & \int \cos(x) \, dx &= \sin(x) + C \\
& & \int \tan(x) \, dx &= -\ln|\cos(x)| + C \\
& & \int \cot(x) \, dx &= \ln|\sin(x)| + C \\
& & \int \sec(x) \, dx &= \ln|\sec(x) + \tan(x)| + C \\
& & \int \csc(x) \, dx &= -\ln|\csc(x) + \cot(x)| + C \\
&\text{(Inverse Trigonometric Functions)} & \int \frac{1}{\sqrt{1-x^2}} \, dx &= \sin^{-1}(x) + C \\
& & \int \frac{-1}{\sqrt{1-x^2}} \, dx &= \cos^{-1}(x) + C \\
& & \int \frac{1}{1+x^2} \, dx &= \tan^{-1}(x) + C \\
& & \int \frac{-1}{1+x^2} \, dx &= \cot^{-1}(x) + C \\
& & \int \frac{1}{x\sqrt{x^2-1}} \, dx &= \sec^{-1}(x) + C \\
& & \int \frac{-1}{x\sqrt{x^2-1}} \, dx &= \csc^{-1}(x) + C
\end{aligned}
$$


### Other

